

# I. Set Theory and Generalized Inclusion-Exclusion

## I.A. Fundamental Set Identities and Cardinality

**Definition 0.1** (Key Set Operations). Let  $A, B$  be sets in a universal set  $U$ .

- (i) **Difference:**  $A \setminus B = A \cap B^c$ .
- (ii) **Symmetric Difference:**  $A \Delta B = (A \setminus B) \cup (B \setminus A) = (A \cup B) \setminus (A \cap B)$ .
- (iii) **Cardinality of Symmetric Difference:**  $|A \Delta B| = |A| + |B| - 2|A \cap B|$ .
- (iv) **De Morgan's Laws (Generalized):**  $(\bigcup_{i=1}^n A_i)^c = \bigcap_{i=1}^n A_i^c$ .

**Theorem 0.1** (PIE for Two and Three Sets). (i)  $|A \cup B| = |A| + |B| - |A \cap B|$ .

(ii)  $|A \cup B \cup C| = |A| + |B| + |C| - (|A \cap B| + |A \cap C| + |B \cap C|) + |A \cap B \cap C|$ .

**Proof (Detailed).**[Proof for Two Sets  $|A \cup B|$ ]  $A \cup B$  can be written as the disjoint union  $A \cup (B \setminus A)$ . By the Sum Rule for disjoint sets:

$$|A \cup B| = |A| + |B \setminus A|$$

Since  $B = (A \cap B) \cup (B \setminus A)$  (disjoint union), we have:

$$|B| = |A \cap B| + |B \setminus A| \implies |B \setminus A| = |B| - |A \cap B|$$

Substituting this back into the first equation yields  $|A \cup B| = |A| + |B| - |A \cap B|$ . ▲

## I.B. Generalized Inclusion-Exclusion

**Theorem 0.2** (Principle of Inclusion-Exclusion (PIE) - General Form). Let  $A_1, A_2, \dots, A_n$  be finite sets. The cardinality of their union is:

$$\left| \bigcup_{i=1}^n A_i \right| = \sum_{k=1}^n (-1)^{k-1} S_k$$

where  $S_k = \sum_{1 \leq i_1 < \dots < i_k \leq n} |A_{i_1} \cap \dots \cap A_{i_k}|$  (the sum of the cardinalities of all  $\binom{n}{k}$  intersections of  $k$  distinct sets).

**Proof (Detailed).**[Detailed Proof of General PIE] Consider an element  $x$ . If  $x$  belongs to exactly  $m \geq 1$  sets, we must show that  $x$  is counted exactly once in the RHS sum.  $x$  is counted in  $S_k$  if

the intersection  $A_{i_1} \cap \dots \cap A_{i_k}$  contains  $x$ . Since  $x$  is in  $m$  sets, there are  $\binom{m}{k}$  such  $k$ -intersections. The net contribution of  $x$  to the RHS is:

$$\sum_{k=1}^m (-1)^{k-1} \binom{m}{k} = 1 - \sum_{k=0}^m (-1)^k \binom{m}{k} = 1 - (1-1)^m$$

Since  $m \geq 1$ ,  $(1-1)^m = 0$ , so the contribution is 1. If  $m = 0$ , the sum is 0. Thus, every element in the union is counted exactly once. ▲

**Theorem 0.3** (Generalized PIE: Exactly  $k$  Elements ( $E_k$ )). Let  $E_k$  be the number of elements belonging to **exactly**  $k$  of the  $n$  sets  $A_1, \dots, A_n$ .

$$E_k = \sum_{j=k}^n (-1)^{j-k} \binom{j}{k} S_j$$

**Proof (Detailed).**[Proof of  $E_k$  Formula] Consider an element  $x$  that belongs to exactly  $m$  sets.

- (a) If  $m < k$ ,  $x$  is not in  $E_k$ , and since  $\binom{j}{k} = 0$  for  $j < k$ , the sum is 0.
- (b) If  $m \geq k$ ,  $x$  is counted 1 time in  $E_k$ .  $x$  contributes to  $S_j$  exactly  $\binom{m}{j}$  times. The total count for  $x$  on the RHS is:

$$\sum_{j=k}^m (-1)^{j-k} \binom{j}{k} \binom{m}{j}$$

Using the identity  $\binom{j}{k} \binom{m}{j} = \binom{m}{k} \binom{m-k}{j-k}$  and letting  $i = j - k$ :

$$\sum_{i=0}^{m-k} (-1)^i \binom{m}{k} \binom{m-k}{i} = \binom{m}{k} \sum_{i=0}^{m-k} (-1)^i \binom{m-k}{i}$$

By the Binomial Theorem,  $\sum_{i=0}^N (-1)^i \binom{N}{i} = (1-1)^N = 0$  for  $N > 0$ . Thus, the total count is  $\binom{m}{k} (1-1)^{m-k}$ , which is 1 if  $m = k$  and 0 if  $m > k$ . This correctly equals  $E_k$ 's contribution. ▲

## II. Advanced Combinatorics and Counting

### II.A. Permutations and Combinations

**Formula 0.1** ( $k$ -Permutations (Ordered, No Repetition)).

$$P(n, k) = \frac{n!}{(n-k)!}$$

**Formula 0.2** ( $k$ -Combinations (Unordered, No Repetition)).

$$\binom{n}{k} = \frac{n!}{k!(n-k)!}$$

**Formula 0.3** (Combinations with Repetition (Multisets)). The number of ways to choose  $k$  items from  $n$  categories with repetition allowed:

$$\text{Multiset } \binom{n}{k} = \binom{n+k-1}{k}$$

**Principle 0.1** (Stars and Bars). The number of non-negative integer solutions to  $x_1 + x_2 + \cdots + x_n = k$  is  $\binom{n+k-1}{k}$ . This is equivalent to arranging  $k$  "stars" and  $n-1$  "bars."

## II.B. Advanced Counting Identities

**Formula 0.4** (Derangements). The number of permutations  $\pi$  of  $n$  objects such that  $\pi(i) \neq i$  for all  $i$  is the number of derangements,  $!n$  (or  $D_n$ ):

$$!n = n! \sum_{k=0}^n \frac{(-1)^k}{k!} = \left\lfloor \frac{n!}{e} + \frac{1}{2} \right\rfloor$$

**Formula 0.5** (Vandermonde's Identity).

$$\binom{r+s}{n} = \sum_{k=0}^n \binom{r}{k} \binom{s}{n-k}$$

**Formula 0.6** (Hockey-Stick Identity).

$$\sum_{i=r}^n \binom{i}{r} = \binom{n+1}{r+1}$$

## II.C. Stirling Numbers

**Definition 0.2** (Stirling Numbers of the Second Kind,  $\left\{ \begin{smallmatrix} n \\ k \end{smallmatrix} \right\}$ ). The number of ways to partition a set of  $n$  distinct objects into  $k$  non-empty, indistinguishable subsets.

**Formula 0.7** (Stirling Numbers of the Second Kind (Explicit Formula)).

$$\left\{ \begin{smallmatrix} n \\ k \end{smallmatrix} \right\} = \frac{1}{k!} \sum_{j=0}^k (-1)^{k-j} \binom{k}{j} j^n$$

**Formula 0.8** (Stirling Numbers of the Second Kind (Recurrence)).

$$\left\{ \begin{smallmatrix} n \\ k \end{smallmatrix} \right\} = \left\{ \begin{smallmatrix} n-1 \\ k-1 \end{smallmatrix} \right\} + k \left\{ \begin{smallmatrix} n-1 \\ k \end{smallmatrix} \right\}$$

**Definition 0.3** (Stirling Numbers of the First Kind (Absolute),  $\left[ \begin{smallmatrix} n \\ k \end{smallmatrix} \right]$ ). The number of permutations of  $n$  distinct objects that have exactly  $k$  disjoint cycles.

**Formula 0.9** (Stirling Numbers of the First Kind (Recurrence)).

$$\left[ \begin{smallmatrix} n \\ k \end{smallmatrix} \right] = \left[ \begin{smallmatrix} n-1 \\ k-1 \end{smallmatrix} \right] + (n-1) \left[ \begin{smallmatrix} n-1 \\ k \end{smallmatrix} \right]$$

## III. Axiomatic Probability and Total Probability

### III.A. Axiomatic Foundations

**Axiom 0.1** (Kolmogorov's Axioms). A probability measure  $\mathbb{P}$  on a sample space  $\Omega$  with  $\sigma$ -algebra  $\mathcal{F}$  satisfies:

- (i) **Non-negativity:**  $\mathbb{P}(A) \geq 0$  for all  $A \in \mathcal{F}$ .
- (ii) **Unit Measure:**  $\mathbb{P}(\Omega) = 1$ .
- (iii) **Countable Additivity:** If  $A_1, A_2, \dots$  are pairwise disjoint events, then  $\mathbb{P}(\bigcup_{i=1}^{\infty} A_i) = \sum_{i=1}^{\infty} \mathbb{P}(A_i)$ .

**Property 0.1** (Derived Properties). (i)  $\mathbb{P}(\emptyset) = 0$ .

(ii)  $\mathbb{P}(A^c) = 1 - \mathbb{P}(A)$ .

(iii) **Monotonicity:** If  $A \subseteq B$ , then  $\mathbb{P}(A) \leq \mathbb{P}(B)$ .

### III.B. Conditional Probability and Independence

**Definition 0.4** (Conditional Probability). For events  $A$  and  $B$  where  $\mathbb{P}(B) > 0$ :

$$\mathbb{P}(A | B) = \frac{\mathbb{P}(A \cap B)}{\mathbb{P}(B)}$$

**Definition 0.5** (Independence). Events  $A$  and  $B$  are independent if and only if:

$$\mathbb{P}(A \cap B) = \mathbb{P}(A) \mathbb{P}(B)$$

**Formula 0.10** (Multiplication Rule (Chain Rule)).

$$\mathbb{P}\left(\bigcap_{i=1}^n A_i\right) = \mathbb{P}(A_1) \mathbb{P}(A_2 | A_1) \mathbb{P}(A_3 | A_1 \cap A_2) \cdots \mathbb{P}\left(A_n | \bigcap_{i=1}^{n-1} A_i\right)$$

**Theorem 0.4** (Law of Total Probability (LTP) - Generalized). If  $B_1, B_2, \dots, B_n$  form a partition of the sample space  $\Omega$  (disjoint, union is  $\Omega$ , and  $\mathbb{P}(B_i) > 0$ ), then for any event  $A$ :

$$\mathbb{P}(A) = \sum_{i=1}^n \mathbb{P}(A | B_i) \mathbb{P}(B_i)$$

## IV. Bayes' Theorem and Generalized Formulae

**Theorem 0.5** (Bayes' Theorem). For events  $A$  and  $B$  (with  $\mathbb{P}(A) > 0, \mathbb{P}(B) > 0$ ):

$$\mathbb{P}(B | A) = \frac{\mathbb{P}(A | B) \mathbb{P}(B)}{\mathbb{P}(A)}$$

**Theorem 0.6** (Generalized Bayes' Theorem for  $N$  Events (Partition)). If  $B_1, B_2, \dots, B_n$  form a partition of the sample space  $\Omega$ , then for any event  $A$  (with  $\mathbb{P}(A) > 0$ ) and any  $j \in \{1, \dots, n\}$ :

$$\mathbb{P}(B_j | A) = \frac{\mathbb{P}(A | B_j) \mathbb{P}(B_j)}{\sum_{i=1}^n \mathbb{P}(A | B_i) \mathbb{P}(B_i)}$$

**Theorem 0.7** (Bayes' Theorem for 3 Events). Specifically, if  $B_1, B_2, B_3$  partition  $\Omega$ :

$$\mathbb{P}(B_1 | A) = \frac{\mathbb{P}(A | B_1) \mathbb{P}(B_1)}{\mathbb{P}(A | B_1) \mathbb{P}(B_1) + \mathbb{P}(A | B_2) \mathbb{P}(B_2) + \mathbb{P}(A | B_3) \mathbb{P}(B_3)}$$

**Proof (Detailed).**[Proof of Generalized Bayes' Theorem] We start with the definition of conditional probability:

$$\mathbb{P}(B_j | A) = \frac{\mathbb{P}(A \cap B_j)}{\mathbb{P}(A)}$$

The numerator,  $\mathbb{P}(A \cap B_j)$ , can be rewritten using the product rule:

$$\mathbb{P}(A \cap B_j) = \mathbb{P}(A | B_j) \mathbb{P}(B_j) \quad (\text{Numerator})$$

The denominator,  $\mathbb{P}(A)$ , can be rewritten using the Law of Total Probability over the partition  $\{B_i\}_{i=1}^n$ :

$$\mathbb{P}(A) = \sum_{i=1}^n \mathbb{P}(A \cap B_i) = \sum_{i=1}^n \mathbb{P}(A | B_i) \mathbb{P}(B_i) \quad (\text{Denominator})$$

Substituting the expressions for the numerator and denominator yields the generalized formula.

▲

## V. Probability Inequalities

### V.A. Bounds on Probability

**Inequality 0.1** (Boole's Inequality (Union Bound)). For any sequence of events  $A_1, A_2, \dots$ :

$$\mathbb{P}\left(\bigcup_{i=1}^{\infty} A_i\right) \leq \sum_{i=1}^{\infty} \mathbb{P}(A_i)$$

**Proof (Detailed).**[Proof of Boole's Inequality] Define a sequence of disjoint events  $B_i$  such that  $\bigcup A_i = \bigcup B_i$ : Let  $B_1 = A_1$ , and for  $i \geq 2$ ,  $B_i = A_i \setminus (\bigcup_{j=1}^{i-1} A_j) = A_i \cap (\bigcap_{j=1}^{i-1} A_j^c)$ . Since the  $B_i$  are disjoint and  $B_i \subseteq A_i$ , we apply Countable Additivity (Axiom iii) and Monotonicity:

$$\mathbb{P}\left(\bigcup_{i=1}^{\infty} A_i\right) = \mathbb{P}\left(\bigcup_{i=1}^{\infty} B_i\right) = \sum_{i=1}^{\infty} \mathbb{P}(B_i)$$

Since  $B_i \subseteq A_i$ ,  $\mathbb{P}(B_i) \leq \mathbb{P}(A_i)$ .

$$\sum_{i=1}^{\infty} \mathbb{P}(B_i) \leq \sum_{i=1}^{\infty} \mathbb{P}(A_i)$$

▲

**Inequality 0.2** (Bonferroni Inequalities). Let  $S_k = \sum_{1 \leq i_1 < \dots < i_k \leq n} \mathbb{P}(A_{i_1} \cap \dots \cap A_{i_k})$  be the  $k$ -th term sum from the probabilistic PIE formula. The probability of the union is bounded by the partial sums:

$$\mathbb{P}\left(\bigcup_{i=1}^n A_i\right) = \sum_{k=1}^n (-1)^{k-1} S_k$$

- (i) **Lower Bound ( $m$  odd):**  $\mathbb{P}(\bigcup_{i=1}^n A_i) \geq \sum_{k=1}^m (-1)^{k-1} S_k$
- (ii) **Upper Bound ( $m$  even):**  $\mathbb{P}(\bigcup_{i=1}^n A_i) \leq \sum_{k=1}^m (-1)^{k-1} S_k$

**Proof (Detailed).**[Proof of Bonferroni Inequalities] The inequalities arise from truncating the alternating series for the PIE. The error term  $R_m = \mathbb{P}(\bigcup A_i) - \sum_{k=1}^m (-1)^{k-1} S_k$  is equal to:

$$R_m = \sum_{k=m+1}^n (-1)^{k-1} S_k = (-1)^m \sum_{k=m+1}^n (-1)^{k-(m+1)} S_k$$

By the generalized PIE for  $E_{m+1}$  (the probability that \*exactly\*  $m+1$  events occur), one can show that the remaining sum  $\sum_{k=m+1}^n (-1)^{k-(m+1)} S_k$  has the same sign as the first term  $S_{m+1}$ , and in fact, is equivalent to the probability that at least  $m+1$  events occur (which is non-negative).

$$R_m = (-1)^m \mathbb{P}(\text{at least } m+1 \text{ events occur})$$

- (a) If  $m$  is odd,  $R_m \leq 0$ , hence  $\mathbb{P}(\bigcup A_i) \leq \sum_{k=1}^m (-1)^{k-1} S_k$ . (Wait, this is  $R_m = \mathbb{P}(\bigcup A_i) - \text{Lower Bound}$ , so  $\mathbb{P}(\bigcup A_i) \leq \text{Lower Bound}$  is wrong. Let's redefine the signs.) The error term should be defined in terms of  $E_{\geq m+1}$ , the probability that at least  $m+1$  events occur. Let  $P(k)$  be the probability that exactly  $k$  events occur.  $P(k) = \sum_{j=k}^n (-1)^{j-k} \binom{j}{k} S_j$ .  $\mathbb{P}(\bigcup A_i) = \sum_{k=1}^n P(k)$ . The remainder  $R_m = \mathbb{P}(\bigcup A_i) - \sum_{k=1}^m (-1)^{k-1} S_k$ . It can be shown that  $(-1)^{m+1} R_m \geq 0$ .
- (b) If  $m$  is odd ( $m+1$  is even),  $R_m \geq 0$ , so  $\mathbb{P}(\bigcup A_i) \geq \sum_{k=1}^m (-1)^{k-1} S_k$ .
- (c) If  $m$  is even ( $m+1$  is odd),  $R_m \leq 0$ , so  $\mathbb{P}(\bigcup A_i) \leq \sum_{k=1}^m (-1)^{k-1} S_k$ .

▲

## V.B. Moment Inequalities

**Inequality 0.3** (Markov's Inequality). If  $X$  is a non-negative random variable ( $X \geq 0$ ) and  $a > 0$ , then:

$$\mathbb{P}(X \geq a) \leq \frac{\mathbb{E}[X]}{a}$$

**Proof (Detailed).**[Proof of Markov's Inequality (Continuous Case)] Assume  $X$  has a probability density function  $f(x)$ . Since  $X \geq 0$ :

$$\mathbb{E}[X] = \int_0^\infty x f(x) dx$$

We split the integral at  $a$ :

$$\mathbb{E}[X] = \int_0^a xf(x)dx + \int_a^\infty xf(x)dx$$

Since  $x \geq 0$ ,  $\int_0^a xf(x)dx \geq 0$ . Also, for  $x \in [a, \infty)$ ,  $x \geq a$ .

$$\mathbb{E}[X] \geq \int_a^\infty xf(x)dx \geq \int_a^\infty af(x)dx$$

Factoring out  $a$ :

$$\mathbb{E}[X] \geq a \int_a^\infty f(x)dx = a\mathbb{P}(X \geq a)$$

Dividing by  $a$  yields the result. ▲

**Inequality 0.4** (Chebyshev's Inequality). For any random variable  $X$  with finite mean  $\mu = \mathbb{E}[X]$  and finite variance  $\sigma^2 = \text{Var}(X)$ , and for any  $\epsilon > 0$ :

$$\mathbb{P}(|X - \mu| \geq \epsilon) \leq \frac{\sigma^2}{\epsilon^2}$$

**Proof (Detailed).**[Proof of Chebyshev's Inequality] Define the non-negative random variable  $Y = (X - \mu)^2$ . Then  $\mathbb{E}[Y] = \mathbb{E}[(X - \mu)^2] = \text{Var}(X) = \sigma^2$ . The event  $|X - \mu| \geq \epsilon$  is equivalent to  $(X - \mu)^2 \geq \epsilon^2$ . We apply Markov's inequality to  $Y$  with  $a = \epsilon^2$ :

$$\mathbb{P}(Y \geq a) \leq \frac{\mathbb{E}[Y]}{a}$$

Substituting the terms:

$$\mathbb{P}((X - \mu)^2 \geq \epsilon^2) \leq \frac{\mathbb{E}[(X - \mu)^2]}{\epsilon^2} = \frac{\sigma^2}{\epsilon^2}$$

Since  $\mathbb{P}((X - \mu)^2 \geq \epsilon^2) = \mathbb{P}(|X - \mu| \geq \epsilon)$ , the inequality holds. ▲